theories/multiparty/theorems.v
@@ -1,0 +1,59 @@
+From diris.multiparty Require Import invariant langdef progress.
+Require Import Coq.Logic.Classical.
+
+(* This file contains the main theorems about MPGV. *)
+(* This is the theorems part of section 5 in the paper. *)
+
+(* The definitions used in this file can be found in definitions.v *)
+(* The language definition can be found in langdef.v *)
+
+(* Theorem 5.1 *)
+Theorem global_progress e es h :
+  typed ∅ e UnitT -> steps [e] ∅ es h ->
+  (∃ es' h', step es h es' h') ∨ (h = ∅ ∧ ∀ e, e ∈ es -> e = Val UnitV).
+Proof.
+  intros. edestruct inv_global_progress; eauto using invariant_holds.
+Qed.
+
+(* Theorem 5.2 *)
+Theorem reachability_deadlock_freedom es h :
+  deadlock_free es h <-> fully_reachable es h.
+Proof.
+  unfold deadlock_free, fully_reachable.
+  split.
+  - intros. destruct (classic (reachable es h x)); eauto.
+    assert (∃ s : gset object, ∀ x, x ∈ s <-> active es h x ∧ ¬ reachable es h x) as [s Hs].
+    { edestruct activeset_exists. eapply subset_exists. naive_solver. }
+    exfalso. eapply (H s).
+    split; eauto.
+    + set_solver.
+    + naive_solver.
+    + intros ???. assert (¬ reachable es h (Thread i)) by naive_solver.
+      eauto using reachable.
+    + intros ????.
+      destruct (classic (Chan c ∈ s)); eauto. exfalso.
+      eapply Hs in H2 as [].
+      destruct (classic (reachable es h (Chan c))); eauto using reachable.
+      assert (active es h (Chan c)).
+      { destruct H3 as (?&?&?&?&?&?&?&?). eexists. eauto. }
+      naive_solver.
+    + intros. apply Hs in H2 as [].
+      rewrite Hs.
+      split. { by eapply obj_refs_active. }
+      intro. eapply H4.
+      eauto using reachable.
+  - intros. intros [].
+    eapply set_choose_L in dl_nonempty as [x Hx].
+    assert (reachable es h x) as Q by eauto.
+    induction Q; naive_solver.
+Qed.
+
+(* Theorem 5.3 *)
+Theorem deadlock_freedom_and_full_reachability e es h :
+  typed ∅ e UnitT -> steps [e] ∅ es h ->
+  deadlock_free es h ∧ fully_reachable es h.
+Proof.
+  intros Htyped Hinv%invariant_holds; last done.
+  split; [eapply reachability_deadlock_freedom|];
+  unfold fully_reachable; eauto using strong_progress.
+Qed.
