README.md
@@ -1,16 +1,26 @@
 # Connectivity Graphs Coq Development
 
 This is the repository for the Connectivity Graphs Coq development.
-Connectivity graphs are a method for progress and preservation style deadlock and memory leak freedom proofs for languages in which these properties are guaranteed by the type system, such as session typed languages.
+The individual components are in the subfolders of the `theories` folder:
+* theories/cgraphs: the generic connectivity graphs library on which the other developments are based.
+* theories/sessiontypes: deadlock freedom for binary session types.
+* theories/multiparty: deadlock freedom for MPGV multiparty session types.
+* theories/lambdabar: deadlock freedom for a language with synchronous barriers.
+
+The subfolders contain documentation for each of the individual developments.
+
 
 To build the code, install the following dependencies:
 
-* A recent version of Coq (we tested with Coq 8.13.2)
-* A development version of Iris (we tested with dev.2021-09-27.1.d2c226e7)
-* A development version of std++ (we tested with dev.2021-09-27.0.7d5f3593)
+* Coq (we tested with Coq 8.15.1)
+* std++ (we tested with dev.2022-05-16.1.411eb445)
+* Iris (we tested with dev.2022-05-25.0.d46e4472)
+
+We recommend installing the `opam` package manager, and then installing the `coq-iris` package as follows:
+
+    opam repo add coq-released https://coq.inria.fr/opam/released
+    opam install coq-iris
+
+This will install the required dependencies.
 
 You can then compile this project with `make`.
-
-The theories folder contains the code for each of the subcomponents and their documentation.
-
-See cgraphs.pdf for more detailed information.
