theories/multiparty/README.md
@@ -1,0 +1,38 @@
+MPGV: multiparty session types
+===============================
+
+This is the Coq development of MPGV.
+This development proves the main theorems that MPGV satisfies:
+- Global progress
+- Deadlock freedom
+- Full reachability (memory leak freedom)
+
+The files of interest are:
+- langdef.v: Definition of the MPGV language (syntax + operational semantics + type system).
+- globaltypes.v: The definition of global types, and proof that global type consistency implies coinductive consistency.
+- binary.v: Encoding binary session types in MPGV.
+- definitions.v: Definitions required to formulate the main theorems (mainly, definition of deadlock freedom and full reachability).
+- theorems.v: The proofs of the main theorems (global progress, deadlock freedom, and full reachability).
+
+The correspondence between these files and the paper is as follows:
+- langdef.v: Section 3
+- globaltypes.v: Section 3.2.
+-  binary.v: Section 4
+- definitions.v: First half of section 5 (the definitions)
+- theorems.v: Second half of section 5 (the theorems)
+
+The other files in this folder contain internal details of the proofs.
+These files are checked by Coq and hence need not be checked to verify the correctness of the theorems.
+- rtypesystem.v: Run-time type system of MPGV.
+- invariant.v: Definition of the configuration invariant and various lemmas about it.
+- progress.v: Lemmas showing that the invariant implies strong progress. These lemmas are used by theorems.v.
+- ycombinator.v: Definition of the y-combinator that can be used to build recursive functions.
+- mutil.v: Various utilities and imports.
+
+# Difference between the paper and Coq
+
+The Coq development is slightly more general than the paper.
+In Coq, we first define a coinductive consistency relation (called [consistent] in Coq).
+We then prove that this implies the consistency notion used in the paper (called [consistent_gt] in Coq), which uses global types.
+This is stronger than what is in the paper, because we can potentially type check more programs using [consistent] than with [consistent_gt].
+The reviewers asked for this change, and in the final version of the paper we will also use these two notions of consistency, like we already do in Coq.
